Logic/Modal/Standard/Kripke/Soundness.lean
@@ -10,14 +10,14 @@ open Formula
 
 open DeductionParameter (Normal)
 
-lemma sound [definability : Ax.DefinesKripkeFrameClass 𝔽] (d : Axᴺ ⊢! p) : 𝔽 ⊧ p := by
+lemma sound (defines : Ax.DefinesKripkeFrameClass 𝔽) (d : Axᴺ ⊢! p) : 𝔽 ⊧ p := by
   induction d using Deduction.inducition_with_necOnly! with
   | hMaxm h =>
     simp only [Set.mem_setOf_eq] at h;
     rcases h with (hK | hR);
     . exact (Semantics.RealizeSet.setOf_iff.mp valid_on_KripkeFrameClass.axiomK) _ hK;
     . intro F hF;
-      exact Semantics.RealizeSet.setOf_iff.mp (definability.defines.mpr hF) _ hR;
+      exact Semantics.RealizeSet.setOf_iff.mp (defines.mpr hF) _ hR;
   | hMdp ihpq ihp => exact valid_on_KripkeFrameClass.mdp ihpq ihp;
   | hNec ih => exact valid_on_KripkeFrameClass.nec ih;
   | hDisj₃ =>
@@ -28,29 +28,28 @@ lemma sound [definability : Ax.DefinesKripkeFrameClass 𝔽] (d : Axᴺ ⊢! p) 
     | inr hq => exact hqr hq;
   | _ => simp_all [valid_on_KripkeFrameClass, valid_on_KripkeFrame, valid_on_KripkeModel, kripke_satisfies];
 
-instance instSound [Ax.DefinesKripkeFrameClass 𝔽] : Sound Axᴺ 𝔽 := ⟨sound⟩
+lemma sound_of_defines (defines : Ax.DefinesKripkeFrameClass 𝔽) : Sound Axᴺ 𝔽 := ⟨sound defines⟩
 
-instance : Sound 𝐊 (AllFrameClass α) := by
-  simpa [←Normal.isK] using (instSound (Ax := 𝗞) (𝔽 := AllFrameClass α));
+instance : Sound 𝐊 (AllFrameClass α) := by simpa [←Normal.isK] using (sound_of_defines (Ax := 𝗞) (𝔽 := AllFrameClass α) axiomK_defines);
 
 
-lemma unprovable_bot (𝔽 : FrameClass α) [Ax.DefinesKripkeFrameClass 𝔽] [nonempty : 𝔽.IsNonempty] : Axᴺ ⊬! ⊥ := by
+lemma unprovable_bot_of_nonempty_frameClass (defines : Ax.DefinesKripkeFrameClass 𝔽) [nonempty : 𝔽.IsNonempty] : Axᴺ ⊬! ⊥ := by
   by_contra hC;
   obtain ⟨F, hF⟩ := nonempty.nonempty
-  simpa using sound hC F hF;
+  simpa using sound defines hC F hF;
 
-lemma consistent (𝔽 : FrameClass α) [Ax.DefinesKripkeFrameClass 𝔽] [𝔽.IsNonempty] : System.Consistent Axᴺ := by
+lemma consistent_of_defines (defines : Ax.DefinesKripkeFrameClass 𝔽) [𝔽.IsNonempty] : System.Consistent Axᴺ := by
   apply System.Consistent.of_unprovable;
-  exact unprovable_bot 𝔽;
+  exact unprovable_bot_of_nonempty_frameClass defines;
 
-private instance instConsistent_of_K' : System.Consistent (𝗞ᴺ : DeductionParameter α) := consistent (𝔽 := AllFrameClass α)
+instance K_consistent' : System.Consistent (𝗞 : AxiomSet α)ᴺ := consistent_of_defines axiomK_defines
 
-instance instConsistent_of_K : System.Consistent (𝐊 : DeductionParameter α) := by
-  simpa [←Normal.isK] using instConsistent_of_K';
+instance K_consistent : System.Consistent (𝐊 : DeductionParameter α) := by
+  simpa [←Normal.isK] using K_consistent';
 
 
 
-lemma finite_sound [definability : Ax.DefinesFiniteKripkeFrameClass 𝔽] (d : Axᴺ ⊢! p) : 𝔽ᶠ ⊧ p := by
+lemma finite_sound (defines : Ax.FinitelyDefinesKripkeFrameClass 𝔽) (d : Axᴺ ⊢! p) : 𝔽ᶠ ⊧ p := by
   induction d using Deduction.inducition_with_necOnly! with
   | hMaxm h =>
     simp only [Set.mem_setOf_eq] at h;
@@ -58,7 +57,7 @@ lemma finite_sound [definability : Ax.DefinesFiniteKripkeFrameClass 𝔽] (d : A
     . exact (Semantics.RealizeSet.setOf_iff.mp valid_on_KripkeFrameClass.axiomK) _ hK;
     . intro F hF;
       simp [FrameClass.toFinite] at hF;
-      apply Semantics.RealizeSet.setOf_iff.mp (definability.defines hF.2 |>.mpr hF.1) _ hR;
+      apply Semantics.RealizeSet.setOf_iff.mp (defines hF.2 |>.mpr hF.1) _ hR;
   | hMdp ihpq ihp => exact valid_on_KripkeFrameClass.mdp ihpq ihp;
   | hNec ih => exact valid_on_KripkeFrameClass.nec ih;
   | hDisj₃ =>
@@ -69,15 +68,15 @@ lemma finite_sound [definability : Ax.DefinesFiniteKripkeFrameClass 𝔽] (d : A
     | inr hq => exact hqr hq;
   | _ => simp_all [valid_on_KripkeFrameClass, valid_on_KripkeFrame, valid_on_KripkeModel, kripke_satisfies];
 
-instance instFiniteSound [Ax.DefinesFiniteKripkeFrameClass 𝔽] : Sound Axᴺ 𝔽ᶠ := ⟨finite_sound⟩
+lemma sound_of_finitely_defines (defines : Ax.FinitelyDefinesKripkeFrameClass 𝔽) : Sound Axᴺ 𝔽ᶠ := ⟨finite_sound defines⟩
 
-lemma unprovable_bot_finite (𝔽 : FrameClass α) [Ax.DefinesFiniteKripkeFrameClass 𝔽] [nonempty : 𝔽ᶠ.IsNonempty] : Axᴺ ⊬! ⊥ := by
+lemma unprovable_bot_of_nonempty_finite_frameClass (defines : Ax.FinitelyDefinesKripkeFrameClass 𝔽) [nonempty : 𝔽ᶠ.IsNonempty] : Axᴺ ⊬! ⊥ := by
   by_contra hC;
   obtain ⟨F, hF⟩ := nonempty.nonempty;
-  simpa using finite_sound hC F hF;
+  simpa using finite_sound defines hC F hF;
 
-lemma consistent_finite (𝔽 : FrameClass α) [Ax.DefinesFiniteKripkeFrameClass 𝔽] [𝔽ᶠ.IsNonempty] : System.Consistent Axᴺ := by
+lemma consistent_of_finitely_defines (defines : Ax.FinitelyDefinesKripkeFrameClass 𝔽) [𝔽ᶠ.IsNonempty] : System.Consistent Axᴺ := by
   apply System.Consistent.of_unprovable;
-  exact unprovable_bot_finite 𝔽;
+  exact unprovable_bot_of_nonempty_finite_frameClass defines;
 
 end LO.Modal.Standard.Kripke
