Logic/Modal/Standard/Kripke/Ver.lean
@@ -14,15 +14,16 @@ variable {α} [Inhabited α] [DecidableEq α]
 
 abbrev IsolatedFrameClass (α) : FrameClass α := { F | Isolated F }
 
-instance : 𝗩𝗲𝗿.DefinesKripkeFrameClass (IsolatedFrameClass α) where
-  defines := by
-    simp [valid_on_KripkeFrame, valid_on_KripkeModel, Isolated];
-    intro F;
-    constructor;
-    . intro h x y hxy;
-      exact h ⊥ (λ _ _ => True) x hxy;
-    . intro hIrrefl p V x y hxy;
-      simp_all;
+lemma axiomVer_defines : 𝗩𝗲𝗿.DefinesKripkeFrameClass (IsolatedFrameClass α)  := by
+  -- simp [valid_on_KripkeFrame, valid_on_KripkeModel, Isolated];
+  simp [AxiomSet.DefinesKripkeFrameClass, valid_on_KripkeFrame];
+  intro F;
+  constructor;
+  . intro h x y hxy;
+    exact h ⊥ (λ _ _ => True) x hxy;
+  . intro hIrrefl _ _ x y hxy;
+    have := hIrrefl hxy;
+    contradiction;
 
 instance : (IsolatedFrameClass α).IsNonempty where
   nonempty := by
@@ -30,14 +31,14 @@ instance : (IsolatedFrameClass α).IsNonempty where
     simp [Isolated];
 
 
-instance : System.Consistent (𝐕𝐞𝐫 : DeductionParameter α) := consistent (𝔽 := IsolatedFrameClass α)
+instance : System.Consistent (𝐕𝐞𝐫 : DeductionParameter α) := consistent_of_defines axiomVer_defines
 
-lemma isolated_CanonicalFrame {Λ : AxiomSet α} (h : 𝗩𝗲𝗿 ⊆ Λ) [System.Consistent Λᴺ] : Isolated (CanonicalFrame Λ) := by
+lemma isolated_CanonicalFrame {Ax : AxiomSet α} (h : 𝗩𝗲𝗿 ⊆ Ax) [System.Consistent Axᴺ] : Isolated (CanonicalFrame Ax) := by
   intro x y rxy;
-  have : (CanonicalModel (α := α) Λ) ⊧ □⊥ := iff_valid_on_canonicalModel_deducible.mpr $ Normal.maxm_ax! (by aesop);
+  have : (CanonicalModel Ax) ⊧ □⊥ := iff_valid_on_canonicalModel_deducible.mpr $ Normal.maxm_ax! (by aesop);
   simp [valid_on_KripkeModel, kripke_satisfies] at this;
-  obtain ⟨p, ⟨hx, hy⟩⟩ := @this x y;
-  have := rxy hx;
+  obtain ⟨_, ⟨hx, hy⟩⟩ := @this x y;
+  have hny := rxy hx;
   contradiction;
 
 instance : Complete (𝐕𝐞𝐫 : DeductionParameter α) (IsolatedFrameClass α) := instComplete_of_mem_canonicalFrame $ isolated_CanonicalFrame (by rfl)
